

Analysis of Algorithms

Lab 02

Name: Santiago Fernando Aispur

Date: 08/10/21/2026

1. Solve the following recurrences. The solution of each exercise includes finding the closed form and then verifying using mathematical induction.

1.1 $T(n) = 3T(n/2) + n$

$T(1) = 0, \forall n \in 2^k, k > 0$

Base case $T(1) = 0$, tell us that we have to find the pattern in order to find the solution, where $T(i), i = 2, 4, 8, 16, \dots$

1) $T(2) = 3T(1) + 2;$

$T(2) = 3T(1) + 2;$

$T(2) = 3(0) + 2;$

$T(2) = 2$

3) $T(8) = 3T(4) + 8;$

$T(8) = 30 + 8;$

$T(8) = 38$

2) $T(4) = 3T(2) + 4;$

$T(4) = 3T(2) + 4;$

$T(4) = 3(2) + 4;$

$T(4) = 10$

4) $T(16) = 3T(8) + 16$

$T(16) = 3(38) + 16$

$T(16) = 130$

Thus if we divide n by 2 on the function, we have got:

$$T\left(\frac{n}{2}\right) = 3T\left(\frac{n}{4}\right) + \frac{n}{2} \Rightarrow T\left(\frac{n}{2}\right) = 3T\left(\frac{n}{4}\right) + \frac{n}{2} \quad (1)$$

if we substitute (1) in $T(n) = 3T(n/2) + n$, we get

$$T(n) = 3\left(3T\left(\frac{n}{4}\right) + \frac{n}{2}\right) + n;$$

$$T(n) = 9T\left(\frac{n}{4}\right) + \frac{3n}{2} + \frac{3n}{2};$$

$$T(n) = 9T\left(\frac{n}{4}\right) + \frac{6n}{2}$$

Thus

If we continue with this substituting pattern until $T(0)$, we will get:

$$T(n) = 2T(3T(0) + \frac{n}{2}) + \frac{n}{4} + \frac{3n}{2} + n;$$

Therefore

$$T(n) = 3^n \cdot T(0) + n \left[1 + \frac{3}{2} + \left(\frac{3}{2}\right)^2 + \left(\frac{3}{2}\right)^3 + \dots + \left(\frac{3}{2}\right)^{n-1} \right]$$

Thus, since $T(0) = 0$

$$T(n) = n \cdot \sum_{j=0}^{n-1} \left(\frac{3}{2}\right)^j \quad \text{by inductive hypothesis}$$

$$1.2 \quad T(n) = 3T(n-1) + 4T(n-2), \quad T(0) = 0, \quad T(1) = 5$$

Base case:

It's given that $T(0) = 0 \wedge T(1) = 5 \quad \forall n > 1$

$$T(2) = 3T(2-1) + 4T(2-2);$$

$$T(2) = 3T(1) + 4T(0);$$

$$T(2) = 3(5) + 4(0);$$

$$T(2) = 15 //$$

$$T(3) = 3T(2) + 4T(1)$$

$$T(3) = 3(15) + 4(5)$$

$$T(3) = 45 + 20 = 65$$

$$T(4) = 3T(3) + 4T(2)$$

$$T(4) = 3(65) + 4(15) = 255$$

Inductive case:

Since the pattern has been found we will use the characteristic equation.

So $T(n) = 3T(n-1) + 4T(n-2)$, becomes

$$r^2 = 3r + 4;$$

$$r^2 - 3r - 4 = 0;$$

$$(r-4)(r+1) = 0;$$

$$r_1 = 4 \wedge r_2 = -1$$

Thus, $T(n) = A(4^n) + B(-1)^n$

After evaluating on initial condition, we get:

$$\begin{aligned} A + B &= 0 \\ 9A - B &= 5 \end{aligned}$$

Since $A = -B$, then:

$$\begin{aligned} 4(-B) - B &= 5 \\ -5B &= 5 \\ B &= -1 \end{aligned}$$

thus $A = 1$

By inductive hypothesis:

So for a $k > 1$, $k \in \mathbb{Z}$:

assuming $T(k) = 4^k - (-1)^k$ is valid.

then for a $k+1$:

$$T(k+1) = 3 \times T(k+1-1) + 4T(k+1-2)$$

$$T(k+1) = 3T(k) + 4T(k-1)$$

$$T(k+1) = 3[4^k - (-1)^k] + 4[4^{k-1} - (-1)^{k-1}]$$

Simplifying

$$T(k+1) = [3 \times 4^k + 4 \times 4^{k-1}] - [3 \times (-1)^k + 4 \times (-1)^{k-1}]$$

$$T(k+1) = 4^{k+1} + (-1)^{k+1} \quad \wedge \quad T(k+1) = 4^{k+1} - (-1)^{k+1}$$

by mathematical induction is correct for all $n > 1$.

$$1.3 \quad T(n) = 5T(n-1) - 6T(n-2), \quad T(0) = 0 \quad T(1) = 1$$

$\forall n \in \mathbb{Z}, n \geq 1.$

Given $T(0) = 0$ & $T(1) = 1$, we will evaluate on $T(n) = 5T(n-1) - 6T(n-2)$

$$T(2) = 5(T(1)) - 6(T(0));$$

$$T(2) = 5(1) - 6(0);$$

$$T(2) = 5;$$

$$T(3) = 5T(2) - 6T(1)$$

$$T(3) = 25 - 6$$

$$T(3) = 19$$

$$T(4) = 5T(3) - 6T(2)$$

$$T(4) = 5(19) - 6(5)$$

$$T(4) = 65$$

Base case

$$T(2) = 5;$$

We will use the characteristic equation as before:

$T(n) = 5T(n-1) - 6T(n-2)$ becomes:

$$r^2 = 5r - 6;$$

$$r^2 - 5r + 6;$$

$$(r-2)(r-3) = 0$$

$$r_1 = 2 \quad \wedge \quad r_2 = 3$$

Therefore

$$T(n) = A \cdot 2^n + B \cdot 3^n$$

So after evaluating on initial conditions:

$$A + B = 0 \quad (T(0))$$

$$2A + 3B = 1 \quad (T(1))$$

Since $A = -B$, then

$$2(-B) + 3B = 1$$

$$B = 1$$

thus $A = -1$;

The CF will be $3^n - 2^n$

Inductive case:

Assume that $\forall k \in \mathbb{Z}$, $k > 1$ then if $k-1$ or $k-2$, then:

$$T(k-1) = 3^{k-1} - 2^{k-1}$$

$$T(k-2) = 3^{k-2} - 2^{k-2}$$

Since $T(k) = 5T(k-1) + 6T(k-2)$, then:

$$T(k) = 5[3^{k-1} - 2^{k-1}] + 6[3^{k-2} - 2^{k-2}]$$

$$T(k) = 5 \cdot 3^{k-1} - 5 \cdot 2^{k-1} + 6 \cdot 3^{k-2} - 6 \cdot 2^{k-2}$$

$$T(k) = 5 \cdot 3^{k-1} + 6 \cdot 3^{k-2} + (-5 \cdot 2^{k-1} - 6 \cdot 2^{k-2})$$

$$T(k) = 5 \cdot 3^k \cdot 3^{-1} + 6 \cdot 3^k \cdot 3^{-2} + (-5 \cdot 2^k \cdot 2^{-1} - 6 \cdot 2^k \cdot 2^{-2})$$

$$T(k) = 3^k \left(\frac{5}{3} + \frac{6}{9} \right) + \left(-2^k \left(\frac{5}{2} + \frac{6}{4} \right) \right)$$

$$T(k) = 3^k - 2^k$$

by inductive hypothesis, $T(n)$ is correct.

$$1.4 \quad x(n) = 2x(n-1) + 4x(n-2), \quad x(0) = 1, \quad x(1) = 2$$

$x > 1$.

As before there is a pattern when viewing $x(i)$ where $i \in \mathbb{Z}$ and $i > 1$. Thus using the characteristic equation, then:

$$x(n) = 2x(n-1) + 4x(n-2) \Rightarrow r^2 = 2r + 4$$

where, $r^2 - 2r - 4 = 0$, then by factorization \Rightarrow

$$r_1 = 2 + \frac{2\sqrt{5}}{2} \wedge r_2 = 2 - \frac{2\sqrt{5}}{2}$$

So $x(n) = A^x (1 + \sqrt{5})^n + B (1 - \sqrt{5})^n$, after evaluating the initial conditions, we have got:

$$\begin{aligned} A + B &= 1 \\ A - B &= 1/\sqrt{5} \end{aligned}$$

Since $A = 1 - B$, then:

$$(1 - B) - B = 1/\sqrt{5};$$

$$1 - 2B = \frac{1}{\sqrt{5}}$$

$$-2B = \frac{1}{\sqrt{5}} - \frac{\sqrt{5}}{\sqrt{5}}$$

$$-2B = \frac{-\sqrt{5}}{\sqrt{5}}$$

$$B = \frac{\sqrt{5}}{2\sqrt{5}}; \text{ thus } A = \frac{\sqrt{5}}{2\sqrt{5}} - \frac{2\sqrt{5}}{2\sqrt{5}} = \frac{2\sqrt{5}}{4\sqrt{5}} = \frac{-\sqrt{5}}{2\sqrt{5}}$$

Assuming $x(k) = 2x(k-1) + 4x(k-2)$ where $k \in \mathbb{Z}$ and $k \geq 1$, then:
if T(k) is valid $x(k+1) = 2x(k) + 4x(k-1)$:

$$\Rightarrow x(k+1) = \left[\frac{-\sqrt{5}}{2\sqrt{5}} \cdot (1 + \sqrt{5})^{k+1} \right] + \left[\frac{\sqrt{5}}{2\sqrt{5}} \cdot (1 - \sqrt{5})^{k+1} \right]$$

By m.i is valid